Try examples from SCT article

examples/mutualwfrec.v
@@ -1,6 +1,6 @@
 From Equations Require Import Equations.
 Require Import Lia.
-Set Transparent Equations.
+Set Equations Transparent.
 Equations evenodd (b : bool) (n : nat) : Prop by rec n lt :=
   evenodd true 0 := True;
   evenodd true (S n) := evenodd false n;
@@ -49,12 +49,12 @@ Polymorphic Equations double_fn {A} {P} (t : ty A P) (x : A) : P x by rec (pack 
   double_fn ty1 (x :: xs) := 0 <? length xs + double_fn ty0 (length xs).
 Next Obligation. Transparent rel. unfold rel. simp rel. cbn. auto with arith. Qed.
 
-Definition fn0 := Eval compute in double_fn ty0.
+Definition fn0 := double_fn ty0.
 Definition fn1 := double_fn ty1.
 
 Lemma fn0_unfold n : fn0 n = n + 0.
 Proof.
-  unfold fn0; simp double_fn.
+  unfold fn0. simp double_fn.
 Qed.
 
 Lemma fn1_unfold l : fn1 l = match l with nil => true | x :: xs => 0 <? length xs + fn0 (length xs) end.
@@ -62,29 +62,121 @@ Proof.
   unfold fn1; simp double_fn. destruct l. simp double_fn. simp double_fn. now rewrite fn0_unfold.
 Qed.
 
-Polymorphic Equations double_fn' {A} {P} (t : ty A P) (x : A) : P x by rec (pack x t) rel :=
-  double_fn' ty0 n := n + 0;
-  double_fn' ty1 l := aux l _
-    where aux l' (H : length l' <= length l)  : _ by struct l' :=
-    aux nil _ := true;
-    aux (x :: xs) H := 0 <? length xs + double_fn' ty0 (length xs) + if aux xs _ then 0 else 1.
-Obligation Tactic := idtac.
-Next Obligation. intros. cbn. auto with arith. Defined.
-Next Obligation. intros. cbn. auto with arith. Defined.
+(* Polymorphic Equations double_fn' {A} {P} (t : ty A P) (x : A) : P x by rec (pack x t) rel := *)
+(*   double_fn' ty0 n := n + 0; *)
+(*   double_fn' ty1 l := aux l _ *)
+(*     where aux l' (H : length l' <= length l)  : _ by struct l' := *)
+(*     aux nil _ := true; *)
+(*     aux (x :: xs) H := 0 <? length xs + double_fn' ty0 (length xs) + if aux xs _ then 0 else 1. *)
+(* Obligation Tactic := idtac. *)
+(* Next Obligation. intros. cbn. auto with arith. Defined. *)
+(* Next Obligation. intros. cbn. auto with arith. Defined. *)
+(* Next Obligation. auto with arith. Defined. *)
+
+(* Definition fn0' := Eval compute in double_fn' ty0. *)
+(* Definition fn1' := double_fn' ty1. *)
+
+(* Lemma fn0'_unfold n : fn0' n = n + 0. *)
+(* Proof. *)
+(*   unfold fn0'; simp double_fn'. *)
+(* Qed. *)
+
+(* Lemma fn1'_unfold l : fn1' l = match l with nil => true | x :: xs => 0 <? length xs + fn0' (length xs) end. *)
+(* Proof. *)
+(*   unfold fn1'; simp double_fn'. destruct l. simp double_fn. simp double_fn'. *)
+(*   destruct double_fn'_unfold_obligation_1. rewrite fn0'_unfold.  auto. *)
+(*   rewrite fn0'_unfold. *)
+(* Admitted. *)
+
+Require Import Equations.Subterm.
+
+Equations ack (m n : nat) : nat by rec (m, n) (lexprod _ _ lt lt) :=
+  ack 0 0         := 1;
+  ack 0 (S n)     := S (S n);
+  ack (S m) 0     := ack m 1;
+  ack (S m) (S n) := ack m (ack (S m) n).
+
+Module Abc.
+
+Inductive abc : Set :=
+| abc0
+  | A (a : abc)
+  | B (b : abc)
+  | C (c : abc).
+
+(* Inductive sct0_rel : abc -> abc -> Prop := *)
+(* | sct0_bc x : sct0_rel (B (C x)) (A x) *)
+(* | sct0_a x : sct0_rel x (A x) *)
+(* | sct0_b x : sct0_rel x (B x) *)
+(* | sct0_c x : sct0_rel x (C x). *)
+(* Hint Constructors sct0_rel : rec_decision. *)
+(* Instance: WellFounded sct0_rel. *)
+(* Admitted. *)
+
+Fixpoint measure_abc (x : abc) :=
+  match x with
+  | abc0 => 0
+  | A x => 3 + measure_abc x
+  | B x => S (measure_abc x)
+  | C x => S (measure_abc x)
+  end.
+
+
+Equations sct0 (x : abc) : nat by rec (measure_abc x) lt :=
+  sct0 abc0 := 0;
+  sct0 (A x) := sct0 (B (C x)) + sct0 x;
+  sct0 (B x) := sct0 x;
+  sct0 (C x) := sct0 x.
+Solve Obligations with program_simpl; lia.
+
+Fixpoint measure_abc' (x : abc) :=
+  match x with
+  | abc0 => 0
+  | A x => S (measure_abc' x)
+  | B x => S (measure_abc' x)
+  | C x => S (measure_abc' x)
+  end.
+
+Equations f1g1 (x : abc) : unit by rec (measure_abc' x) lt :=
+  f1g1 (A (A x)) := f1 x _
+    where f1 x' (H : measure_abc' x' < measure_abc' (A x)) : _ := { f1 x _ := f1g1 (A x) };
+  f1g1 _ := tt.
 Next Obligation. auto with arith. Defined.
 
-Definition fn0' := Eval compute in double_fn' ty0.
-Definition fn1' := double_fn' ty1.
+Equations f1g1' (x : abc) : unit by rec (measure_abc' x) lt :=
+  f1g1' (A (A x)) := f1g1' (A x);
+  f1g1' _ := tt.
+End Abc.
 
-Lemma fn0'_unfold n : fn0' n = n + 0.
-Proof.
-  unfold fn0'; simp double_fn'.
-Qed.
+Module sct2.
 
-Lemma fn1'_unfold l : fn1' l = match l with nil => true | x :: xs => 0 <? length xs + fn0' (length xs) end.
-Proof.
-  unfold fn1'; simp double_fn'. destruct l. simp double_fn. simp double_fn'.
-  destruct double_fn'_unfold_obligation_1. rewrite fn0'_unfold.  auto.
-  rewrite fn0'_unfold.
+  Polymorphic Inductive ty : forall (A : Type) (P : A -> Type), Type :=
+  | ty0 : ty (list nat * list nat)%type (fun _ => list nat)
+  | ty1 : ty (list nat * list nat * list nat) (fun _ => list nat).
 
-Qed.
+  Polymorphic Equations rel' : {A &{ P &{ _ : ty A P & A }}} -> {A & { P & {_ : ty A P & A}}} -> Prop :=
+  rel' &(A', P, ta, a) &(_, Q, tb, b) =>
+  match ta in ty A P, tb in ty B Q return A -> B -> Prop with
+  | ty0, ty0 => fun '(l0, l1) '(l0', l1') => length l0 < length l0'
+  | ty1, ty1 => fun '(l0, n, l1) '(l0', n', l1') => length l0 < length l0'
+  | ty0, ty1 => fun '(l0, l1) '(l0', l1', l2') => length l0 < length l0'
+  | ty1, ty0 => fun l n => True
+  end a b.
+  Transparent rel'.
+  Polymorphic Instance: WellFounded rel'.
+  Proof. Admitted.
+
+
+  Polymorphic Definition pack {A} {P} (t : ty A P) (x : A) :=
+  (&(A, P, t, x)) : {A & {P & {_ : ty A P & A}}}.
+
+  Polymorphic Equations fg {A} {P} (t : ty A P) (x : A) : P x by rec (pack t x) rel' :=
+    fg ty0 (nil, x) := x;
+    fg ty0 (cons y ys, x) := 1 :: fg ty1 (ys, x, (cons y ys));
+    fg ty1 (a, b, c) := 2 :: fg ty0 (a, app b c).
+
+  (* TODO find order! *)
+  Next Obligation. unfold rel'. cbn. exact I. Qed.
+  Next Obligation. unfold rel'. cbn. Admitted.
+
+End sct2.
